# Laziness
Haskell is lazy in how it evaluates programs. 

A very rough outline of Haskell’s evaluation strategy is this: most expressions are only reduced, or evaluated, when necessary. When the evaluation process begins, a thunk is created for each expression.
It means that expressions are not evaluated when they are bound to variables, but their evaluation is deferred until their results are needed by other computations.

In consequence, arguments are not evaluated before they are passed to a function, but only when their values are actually used.

Strict evaluation is where all arguments to a function are evaluated before the body of the function is evaluated; and the arguments are never re-evaluated

## Costs of Lazy Evaluation
* Lazy evaluation has an overhead: building thunks
* Memory consumption per reduction step is typically slightly higher
* In our examples so far:
isOdd (1+2)
len (down 1) we needed to evaluate almost everything
## Benefits of Lazy Evaluation
* Imagine we have a function definition as follows:
        myfun carg struct1 struct2
        = if f carg
        then g struct1
        else h struct2
where f, g and h are internal functions
* Consider the following call:
        myfun val s1Expr s2Expr
where both s1Expr and s2Expr are very expensive to
evaluate.
* With strict evaluation we would have to compute both before applying myfun
* With lazy evaluation we evaluate f val, and then only
evaluate one of either s1Expr or s2Expr,
and then, only if g or h requires its value.

* Prelude function take n xs returns the first n elements of xs
    take 0 _ = []
    take _ [] = []
    take n (x:xs) = x : (take (n-1) xs)
* Function from n generates an infinite ascending list starting with n.
    from n = n : (from (n+1))
* Evaluating from n will fail to terminate for any n.
* Evaluation of take 2 (from 0) depends on the evaluation
method.

## Evaluation Strategy and Termination
We can summarise the relationship between evaluation strategy and termination as:
  * There are programs that simply do not terminate, no matter how they are evaluated
  e.g. from 0
  * There are programs that terminate if evaluated lazily, but fail to terminate if evaluated strictly
  e.g. take 2 (from 0)
  * There are programs that terminate regardless of chosen
  evaluation strategy  e.g. len (down 1)
  * However, there are no programs that terminate if evaluated strictly, but fail to terminate if evaluated lazily




<code>

    Strict evaluation of len (down 1)
    len (down 1)
    = len (if 1 <= 0 then [] else 1 : (down (1-1))
    = len (1 : (down (1-1))
    = len (1 : (down 0))
    = len (1 : (if 0 <= 0 then [] else 0 : (down (0-1))))
    = len (1 : [])
    = if null (1 : []) then 0 else 1 + len (tail (1 : []))
    = 1 + len (tail (1 : []))
    = 1 + len []
    = 1 + len (if null [] then 0 else 1 + len (tail []))
    = 1 + 0
    = 1

    Lazy evaluation of len (down 1) (part 1)
    len (down 1)
    = if null xs1 then 0 else 1 + len (tail xs1)
    where xs1 = down 1
    = if null xs1 then 0 else 1 + len (tail xs1)
    where xs1 = if 1 <= 0 then [] else 1 : (down (1-1))
    = if null xs1 then 0 else 1 + len (tail xs1)
    where xs1 = 1 : (down (1-1))
    = 1 + len (tail xs1) where xs1 = 1 : (down (1-1))
    = 1 + ( if null xs2 then 0 else 1 + len (tail xs2)
    where xs2 = tail xs1 )
    where xs1 = 1 : (down (1-1))

    Lazy evaluation of len (down 1) (part 2)
    1 + ( if null xs2 then 0 else 1 + len (tail xs2)
    where xs2 = tail xs1 )
    where xs1 = 1 : (down (1-1))
    = 1 + ( if null xs2 then 0 else 1 + len (tail xs2)
    where xs2 = tail (1 : (down (1-1))))
    = 1 + ( if null xs2 then 0 else 1 + len (tail xs2)
    where xs2 = down (1-1))
    = 1 + ( if null xs2 then 0 else 1 + len (tail xs2)
    where xs2 = (if (1-1) <= 0
    then [] else (1-1) : (down ((1-1)-1))) )
    = 1 + ( if null xs2 then 0 else 1 + len (tail xs2)
    where xs2 = (if 0 <= 0
    then [] else (1-1): (down ((1-1)-1))) )
    = 1 + ( if null xs2 then 0 else 1 + len (tail xs2)
    where xs2 = [] )
    = 1 + 0
    = 1 12 steps, each more expensive!
</code>

<code>

    take n xs
    take 0 _ = []
    take _ [] = []
    take n (x:xs) = x : (take (n-1) xs)

    from n = n : (from (n+1))


    Strict Evaluation of take 2 (from 0)
    take 2 (from 0)
    = take 2 (0 : from (0+1))
    = take 2 (0 : from 1)
    = take 2 (0 : 1 : from (1+1))
    = take 2 (0 : 1 : from 2)
    = take 2 (0 : 1 : 2 : from (2+1))
    = take 2 (0 : 1 : 2 : from 3)
    = take 2 (0 : 1 : 2 : 3 : from (3+1))
    = take 2 (0 : 1 : 2 : 3 : from 4)
    = take 2 (0 : 1 : 2 : 3 : 4 : from (4+1))
    = take 2 (0 : 1 : 2 : 3 : 4 : from 5)
    = ...

    Lazy Evaluation of take 2 (from 0)
    Here we don’t bother to show the closures explicitly
    (using where xs1 = ...).
    take 2 (from 0)
    = take 2 (0 : from (0+1))
    = 0 : (take (2-1) (from (0+1)))
    = 0 : (take 1 (from (0+1)))
    = 0 : (take 1 ((0+1) : from ((0+1)+1))
    = 0 : (take 1 ((0+1) : from ((0+1)+1)))
    = 0 : (0+1) : (take (1-1) (from ((0+1)+1)))
    = 0 : (0+1) : (take 0 (from ((0+1)+1)))
    = 0 : (0+1) : []
</code>