## Simplifying simp
We can at least isolate the simplifications out:

<code>

    simpOp opsimp e1 e2
    = let e1’ = simp e1
    e2’ = simp e2
    in opsimp e1’ e2’
    simp itself is simpler:
    simp (Add e1 e2) = simpOp addSimp e1 e2
    simp (Mul e1 e2) = simpOp mulSimp e1 e2
    simp (Sub e1 e2) = simpOp subSimp e1 e2
    simp (Dvd e1 e2) = simpOp dvdSimp e1 e2
</code>

* Some operators have nice properties, like having unit values
  
    e.g., 0 + a = a = a + 0 and 1 ∗ a = a = a ∗ 1
* We can code a simplifier for these as follows:


<code>

    uopSimp cons u (Val v) e | v == u = e
    uopSimp cons u e (Val v) | v == u = e
    uopSimp cons u e1 e2 = cons e1 e2
</code>

What is cons here?

* Usage:
  
    simp (Add e1 e2) = uopSimp Add 0.0 e1 e2
    simp (Mul e1 e2) = uopSimp Mul 1.0 e1 e2

### Data Constructors are Functions
The data constructors of Expr, are in fact functions, whose types
are as follows:

<code>

    Val :: Double -> Expr
    Var :: Id -> Expr
    Add :: Expr -> Expr -> Expr
    Mul :: Expr -> Expr -> Expr
    Sub :: Expr -> Expr -> Expr
    Dvd :: Expr -> Expr -> Expr
    Def :: Id -> Expr -> Expr -> Expr

</code>


So, cons on the previous slide needs to have type Expr -> Expr-> Expr, which is why Add and Mul are suitable arguments to pass into uopSimp.


* given declaration
  * data MyType = ... | MyCons T1 T2 ... Tn | ...


* then data constructor MyCons is a function of type
  * MyCons :: T1 -> T2 -> ... -> Tn -> MyType


* Partial applications of MyCons are also valid
  * (MyCons x1 x2) :: T3 -> ... -> Tn -> MyType


* Data constructors are the only functions that can occur in patterns.


# Summary of Abstraction
* process of turning expressions into functions
* if done correctly, greatly increase code re-use and reduces boilerplate

# Higher Order Abstraction
Functions like sum, length, prod all have common pattern referred to as **folding**.

They all have empty list as base case, non empty list as recursive case, base case returns fixed "unit" which we will call *u*. The recursive case combines the head of the list with the result of the recursive call, using a binary operator we shall call *op*.


<code>
    sum [] = 0
    sum (n:ns) = n + sum ns

    length [] = 0
    length (x:xs) = x ‘incr‘ length xs
        where x ‘incr‘ y = 1 + y

    prod [] = 1
    prod (n:ns) = n * prod ns

    < abs-fold > [] = u
    < abs-fold > (a:as) = a ‘op‘ < abs-fold > as
</code>

So we have an abstract form so we make it concrete function fold that takes u and op as arguments.

<code>

    fold u op [] = u
    fold u op (a:as) = a ‘op‘ fold u op as
</code>

## Using fold to save boilerplate code

<code>

    -- sum [] = 0, u = 0
    -- sum (n:ns) = n + sum ns, op = (+)
    sum = fold 0 (+)

    -- length [] = 0, u = 0
    -- length (_:xs) = 1 + length xs, op = incr
    length = fold 0 incr where _ ‘incr‘ y = 1 + y

    -- prod [] = 1, u = 1
    -- prod (n:ns) = n * prod ns, op = (*)
    prod = fold 1 (*)

</code>

## What type is fold?

<code>

    -- a :: t, as :: [t]
    -- u :: r -- result type may differ, e.g. length
    -- op :: t -> r -> r -- 1st from list, 2nd a "result"

    fold :: r -> (t -> r -> r) -> [t] -> r
</code>

Haskell has foldl and foldr. foldr is like ours in that the uses of op are nested on the right.




